\begin{question}
	If $f\circ g$ is surjective, then $f$ is surjective ($P$).

	\begin{proof}

		$$ P_{f\circ g}	\forall x \in X \exists z \in Z : \, (f\circ g)(x) = z $$

		\begin{align*}
			P & = \exists y \in Y \not\exists z \in Z : \, f
		\end{align*}

		\begin{align*}
			P_{f\circ g}\wedge		\neg P   \implies & \exists z \in Z  \forall y \in Y :\, f(y) \neq z     \\
			                                      & \llet x   \in X : \forall z \in Z :\, f(g(x)) \neq z \\
			                                      & \not\exists z \in Z :\, (f\circ g)(x) = z            \\
			\sim                                  & \neg P_{f\circ g}
		\end{align*}

		$$ \neg P \wedge P_{f\circ g} \implies \neg P_{f\circ g} \therefore P $$

	\end{proof}
\end{question}
