\begin{question}

	If $f\circ g$ is injective, then $g$ is injective ($P$).

	\begin{proof}
		$$
			P = \forall x_1,x_2 \in B, g(x_1)=g(x_2) \iff x_1=x_2
		$$

		\begin{align*}
			g: y                   & \mapsto z \\
			f: x                   & \mapsto y \\
			\therefore f\circ g: a & \mapsto c
		\end{align*}

		\begin{align*}
			\neg P & \implies \exists y_0,y_1 \in B :\, g(y_0)=g(y_1) \wedge y_0 = y_1 \\
			       & \implies (f \circ g)(x_0) = f( y_0 ) = f(y_1)
		\end{align*}
	\end{proof}
\end{question}
